examples/ExtensibleIndexes/Classifier.v
@@ -1,0 +1,179 @@
+Require Import ADTSynthesis.QueryStructure.Automation.AutoDB
+        ADTSynthesis.QueryStructure.Automation.IndexSelection
+        ADTSynthesis.QueryStructure.Specification.SearchTerms.ListPrefix
+        ADTSynthesis.Common.List.UpperBound.
+
+Open Scope list.
+
+(* This is an internet packet classifier example. We model a packet with its ip address and 
+   network protocol. The ADT has one relation (table) named [Rules], which contains classification rules *)
+
+Section Packet.
+  (* an Ip address is a list of ascii each of which represents a group *)
+  Definition Ip := list ascii.
+
+  (* a Protocol can be either tcp or udp *)
+  Inductive Protocol := tcp | udp.
+
+  Lemma Protocol_dec : forall a b : Protocol, {a = b} + {a <> b}.
+  Proof. decide equality. Qed.
+
+  Global Instance Query_eq_Protocol :
+    Query_eq Protocol := {| A_eq_dec := Protocol_dec |}.
+
+  (* a Policy of P is either enforcing some constant P, or accepting any *)
+  Section Packet_Protocol.
+    Variable (P : Type).
+    Context {P_eq_dec : Query_eq P}.
+    
+    Inductive Policy :=
+    | enforce : P -> Policy
+    | wildcard.
+    
+    Definition FollowPolicy (p : Policy) (s : P) :=
+      match p with
+        | enforce p' => p' = s
+        | wildcard => True
+      end.
+    
+    Definition FollowPolicy_dec (p: Policy) (s : P) : {FollowPolicy p s} + {~ FollowPolicy p s}.
+      refine (match p with
+                | enforce p' =>
+                  if A_eq_dec p' s then
+                    left _
+                  else
+                    right _
+                | wildcard => left _
+              end); simpl; intuition eauto. Defined.
+    
+    Global Instance DecideableFollowPolicy {T} (f : T -> Policy) {n}
+    : DecideableEnsemble (fun tup => FollowPolicy (f tup) n) :=
+      {| dec n' :=  ?[FollowPolicy_dec (f n') n] |}. intuition; find_if_inside; intuition. Defined.
+  End Packet_Protocol.
+
+  (* a Packet consists of Ip and Protocol *)
+  Record Packet :=
+    { destination : Ip;
+      protocol : Protocol }.
+
+  (* a Response of a query can be accept, deny, or uncertain *)
+  Inductive Response := Accept | Deny | Uncertain.
+End Packet.
+
+Section ADT.
+  (* Rule schema *)
+  Definition RULES := "Rules".
+  Definition PRIORITY := "Priority".
+  Definition DESTINATION := "Destination".
+  Definition PROTOCOL := "Protocol".
+  Definition ACTION := "Action".
+
+  Definition RuleRecord :=
+    @Tuple <PRIORITY :: nat,
+    DESTINATION :: Ip,
+    PROTOCOL :: Policy Protocol,
+    ACTION :: bool>%Heading.
+
+  Definition ClassifierSchema :=
+  Query Structure Schema
+        [ relation RULES has
+                   schema <PRIORITY :: nat,
+          DESTINATION :: Ip,
+          PROTOCOL :: Policy Protocol,
+          ACTION :: bool> ]
+        enforcing [ ].
+
+  (* probably we should use typeclasses to solve this issue *)
+  Definition priority_lt_dec :
+          forall a b : RuleRecord, sumbool (b!PRIORITY <= a!PRIORITY) (~ b!PRIORITY <= a!PRIORITY)
+    := rel_dec_comm _ (rel_dec_map _ le_dec (fun r : RuleRecord => r!PRIORITY)).
+
+  Definition ClassifierSig : ADTSig :=
+  ADTsignature {
+      Constructor "Init" : unit -> rep,
+      Method "AddRule" : rep x RuleRecord -> rep x bool,
+      Method "DeletePrefix" : rep x Ip -> rep x list RuleRecord,
+      Method "Classify" : rep x Packet -> rep x Response
+    }.
+
+  Definition ClassifierSpec : ADT ClassifierSig :=
+  QueryADTRep ClassifierSchema {
+    Def Constructor "Init" (_ : unit) : rep := empty,
+
+    update "AddRule" (r : RuleRecord) : bool :=
+      Insert r into RULES,
+
+    update "DeletePrefix" (ip : Ip) : list RuleRecord :=
+      Delete r from RULES where IsPrefix r!DESTINATION ip,
+
+    query "Classify" (p : Packet) : Response :=
+      rs <- For (r in RULES)
+            (* the rule's ip must be a prefix of the packet's ip *)
+            Where (IsPrefix r!DESTINATION (destination p) /\
+            (* the rule's protocol must match the packet's protocol *)
+                   FollowPolicy r!PROTOCOL (protocol p))
+            Return r;
+      (* try to choose one rule that has the highest priority *)
+      r <- {{ r in rs | r'!PRIORITY <= r!PRIORITY forall r' }} : RuleRecord;
+      (* return its accept / deny if such rule exists, otherwise uncertain *)
+      Ifopt
+        r as r
+      Then
+        If
+          r!ACTION
+        Then
+          ret Accept
+        Else
+          ret Deny
+      Else
+        ret Uncertain
+  }.
+
+  Theorem ClassifierManual :
+    Sharpened ClassifierSpec.
+  Proof.
+    unfold ClassifierSpec.
+    start honing QueryStructure.
+
+    make simple indexes using [[(FindPrefixIndex, DESTINATION)]].
+
+    hone constructor "Init".
+    { initializer. }
+
+    hone method "AddRule".
+    { insertion. }
+
+    hone method "DeletePrefix".
+    { deletion. }
+
+    (* This method involves complex opertations, such as finding the highest priority rules.
+       Some of the deriviations need to be guided manually *)
+    hone method "Classify".
+    {
+      implement_Query.
+      simplify with monad laws.
+      etransitivity.
+      apply refine_under_bind; intros.
+      - setoid_rewrite (refine_pick_upperbound_ineff _ priority_lt_dec).
+        simplify with monad laws.
+        apply refine_under_bind; intros.
+        refine pick val _; eauto.
+        simplify with monad laws.
+        higher_order_1_reflexivity.
+      - simpl. finish honing.
+    }
+
+    FullySharpenQueryStructure ClassifierSchema Index.
+
+    implement_bag_methods.
+    implement_bag_methods.
+    implement_bag_methods.
+  (* 124 seconds *)
+  Time Defined.
+
+  Definition ClassifierImpl : SharpenedUnderDelegates ClassifierSig.  
+    (* 33 seconds *)
+    Time let Impl := eval simpl in (projT1 ClassifierManual) in
+             exact Impl.
+  Defined.
+End ADT.
